coqimp/contextswitch/proof/WindowOKProof.v
@@ -1,9 +1,9 @@
-Require Import Coqlib.                                       
+Require Import Coqlib.                                                
 Require Import Maps.            
 Require Import LibTactics.   
         
 Require Import Integers.  
-Open Scope Z_scope.        
+Open Scope Z_scope.         
 Import ListNotations.  
    
 Set Asymmetric Patterns.  
@@ -34,6 +34,8 @@ Require Import ctxswitch_spec.
 
 Require Import lemma1.
 
+Require Import SaveUsedWindows.
+
 Open Scope nat.
 Open Scope code_scope.
 Open Scope mem_scope.
@@ -44,6 +46,161 @@ Open Scope mem_scope.
 
 (*+ Lemmas for Inference Rule +*)
 
+(*+ Lemmas for Stack Frame Relation +*)
+Lemma stk_fm_constraint_stable1 :
+  forall l lfp fm1 fm2 fm1' fm2' fm3 fm3' F id vi,
+    length F = 13 -> $ 0 <=ᵤᵢ id <=ᵤᵢ $ 7 -> $ 0 <=ᵤᵢ vi <=ᵤᵢ $ 7 ->
+    get_frame_nth fm2 6 = get_frame_nth fm2' 6 ->
+    get_frame_nth fm3 6 = get_frame_nth fm3' 6 ->
+    stack_frame_constraint' l id (fm1 :: fm2 :: F ++ (fm3 :: nil)) lfp vi ->
+    stack_frame_constraint' l id (fm1' :: fm2' :: F ++ (fm3' :: nil)) lfp vi.
+Proof.
+  intros. 
+  do 14 (try destruct F; simpl in H; tryfalse). 
+  clear H.
+  simpls.
+
+  inversion H4; subst.
+  {
+    eapply frame_invalid; eauto.
+  }
+
+  Ltac solve_get_frame_nth :=
+    match goal with
+    | H : get_frame_nth _ _ = get_frame_nth ?fm ?n |- get_frame_nth ?fm ?n = _ =>
+      rewrite <- H; eauto
+    | _ => idtac
+    end.
+  
+  clear H4.
+  inversion H13; subst.
+  { 
+    eapply frame_valid; eauto; solve_get_frame_nth.
+    eapply frame_invalid; eauto.
+  }
+
+  clear H13. 
+  inversion H15; subst.
+  {
+    do 2 (eapply frame_valid; eauto; solve_get_frame_nth).
+    eapply frame_invalid; eauto.
+  }
+
+  clear H15.
+  inversion H17; subst.
+  {
+    do 3 (eapply frame_valid; eauto; solve_get_frame_nth).
+    eapply frame_invalid; eauto.
+  }
+
+  clear H17.
+  inversion H19; subst.
+  {
+    do 4 (eapply frame_valid; eauto; solve_get_frame_nth).
+    eapply frame_invalid; eauto.
+  }
+
+  clear H19.
+  inversion H21; subst.
+  {
+    do 5 (eapply frame_valid; eauto; solve_get_frame_nth).
+    eapply frame_invalid; eauto.
+  }
+
+  clear H21.
+  inversion H23; subst.
+  {
+    do 6 (eapply frame_valid; eauto; solve_get_frame_nth).
+    eapply frame_invalid; eauto.
+  }
+
+  clear H23.
+  inversion H25; subst.
+  {
+    do 7 (eapply frame_valid; eauto; solve_get_frame_nth).
+    eapply frame_invalid; eauto.
+  }
+
+  clear H25.
+  do 8 (eapply frame_valid; eauto; solve_get_frame_nth).
+Qed.
+
+Lemma stk_fm_save_tail_stable1 :
+  forall F fm fm' cstk1 cstk2 id vi,
+    id <> vi -> length F = 13 -> $ 0 <=ᵤᵢ id <=ᵤᵢ $ 7 -> $ 0 <=ᵤᵢ vi <=ᵤᵢ $ 7 ->
+    stack_frame_save (F ++ (fm :: nil)) cstk1 cstk2 id vi ->
+    stack_frame_save (F ++ (fm' :: nil)) cstk1 cstk2 id vi.
+Proof.
+  intros.
+  do 14 (try destruct F; simpl in H0; tryfalse).
+  clear H0.
+  simpls.
+
+  unfolds stack_frame_save.
+  destruct cstk1, cstk2.
+  simpljoin1.
+  split; eauto.
+
+  inversion H3; subst.
+  {
+    eapply frame_save_end; eauto.
+  }
+
+  clear H3.
+  inversion H11; subst.
+  {
+    do 1 (try eapply frame_save_cons; [solve_post_neq | idtac];
+          repeat (eapply post_cons_neq_still_rev; eauto)).
+    eapply frame_save_end; eauto.
+  }
+
+  clear H11.
+  inversion H12; subst.
+  {
+    do 2 (try eapply frame_save_cons; [solve_post_neq | idtac];
+          repeat (eapply post_cons_neq_still_rev; eauto)).
+    eapply frame_save_end; eauto.
+  }
+
+  clear H12.
+  inversion H13; subst.
+  {
+    do 3 (try eapply frame_save_cons; [solve_post_neq | idtac];
+          repeat (eapply post_cons_neq_still_rev; eauto)).
+    eapply frame_save_end; eauto.
+  }
+
+  clear H13.
+  inversion H14; subst.
+  {
+    do 4 (try eapply frame_save_cons; [solve_post_neq | idtac];
+          repeat (eapply post_cons_neq_still_rev; eauto)).
+    eapply frame_save_end; eauto.
+  }
+
+  clear H14.
+  inversion H15; subst.
+  {
+    do 5 (try eapply frame_save_cons; [solve_post_neq | idtac];
+          repeat (eapply post_cons_neq_still_rev; eauto)).
+    eapply frame_save_end; eauto.
+  }
+
+  clear H15.
+  inversion H16; subst.
+  {
+    do 6 (try eapply frame_save_cons; [solve_post_neq | idtac];
+          repeat (eapply post_cons_neq_still_rev; eauto)).
+    eapply frame_save_end; eauto.
+  }
+
+  inversion H17; subst.
+  clear - H H1.
+  rewrite post_8_eq in H.
+  tryfalse.
+  eauto.
+Qed.
+  
 (*+ Proof +*)
 Theorem Ta0WindowOKProof :
   forall vl,
@@ -73,7 +230,7 @@ Proof.
   
   unfold ta0_window_ok.
   destruct fmg, fmo, fml, fmi.
-  hoare_lift_pre 2.
+  hoare_lift_pre 2. 
 
   eapply backward_rule.
   introv Hs.
@@ -224,7 +381,6 @@ Proof.
   simpl upd_genreg.
  
   (** call reg_save; nop *)
-  clear Hlgvl.
   eapply call_rule.
   {
     eval_spec.
@@ -240,20 +396,21 @@ Proof.
     TimReduce_simpl.
     eapply nop_rule; eauto.
   }
-  {   
+  {    
     unfold reg_save_pre.
     instantiate (1 :=
                    logic_fm ([[ct -ᵢ ($ 0), w0, w1, w2, w3, w4, w5, w6]])
                             :: logic_fm ([[w7, w8, w9, w10, w11, w12, w13, $ 204]])
                             :: logic_fm ([[w15, w16, w17, w18, ct, ct +ᵢ ($ 84), w21, w22]])
                             :: logic_fm ([[w23, w24, w25, w26, w27, w28, w29, w30]])
+                            :: logic_lv ct +ᵢ OS_CONTEXT_OFFSET
                             :: logic_lv id :: logic_lv vi :: logic_fmls F
                             :: logic_lv vy :: logic_lv ($ 204) :: nil).
-    introv Hs. 
+    introv Hs.  
     sep_ex_elim_in Hs.
     eapply sep_pure_l_elim in Hs.
     destruct Hs as [Hlgvl_save Hs].
-    symmetry in Hlgvl_save.
+    symmetry in Hlgvl_save. 
     inversion Hlgvl_save; subst.
     clear Hlgvl_save.
     simpl_sep_liftn_in Hs 5.
@@ -316,7 +473,7 @@ Proof.
   {
     DlyFrameFree_elim.
   }
-
+  
   unfold reg_save_post.
   hoare_ex_intro_pre.
   eapply backward_rule.
@@ -324,10 +481,10 @@ Proof.
   asrt_to_line_in Hs 5.
   eauto.
   eapply Pure_intro_rule.
-  introv Hlgvl.
-  symmetry in Hlgvl.
-  inversion Hlgvl; subst.
-  clear Hlgvl.
+  introv Hlgvl1.
+  symmetry in Hlgvl1.
+  inversion Hlgvl1; subst.
+  clear Hlgvl1.
   renames x'3 to cctx'.
 
   (** getcwp g4 *) 
@@ -371,6 +528,153 @@ Proof.
   introv Hin_range.
   destruct Hin_range as [Hid_inrange Hvi_inrange].
   rewrite get_range_0_4_stable; eauto.
+  destruct Hst_fm_constraint as [Hst_fm_constraint Hpost_valid].
+
+  hoare_lift_pre 5.
+  eapply Pure_intro_rule.
+  introv Hwin_save.
   
-Admitted.
+  eapply hoare_pure_gen' with (pu := length F = 13).
+  {
+    introv Hs.
+    simpl_sep_liftn_in Hs 2.
+    unfold FrameState in Hs.
+    asrt_to_line_in Hs 3.
+    simpl_sep_liftn_in Hs 3.
+    eapply sep_pure_l_elim in Hs.
+    simpljoin1; eauto.
+  }
+  eapply Pure_intro_rule.
+  introv Hlen_F.
+  destruct cstk as [cl clfp].
+  
+  eapply Seq_conseq_rule.
+  eapply Ta0SaveUsedWindowsProof; eauto. 
+
+  introv Hs.
+  unfold ta0_save_usedwindows_pre.  
+  sep_ex_intro. 
+  eapply sep_pure_l_intro; eauto.
+  simpl_sep_liftn 2. 
+  eapply GenRegs_split_Regs_Global.
+  do 2 sep_cancel1 1 1.
+  sep_cancel1 2 1.
+  sep_cancel1 3 1.
+  sep_cancel1 2 1.
+  sep_cancel1 1 5.
+  sep_cancel1 1 1.
+  sep_cancel1 2 1.
+  sep_cancel1 1 2.
+  sep_cancel1 1 1. 
+  sep_cancel1 2 2.
+  sep_cancel1 2 2.
+  assert (Htrivial : clfp = nil ++ clfp).
+  eauto. 
+  match goal with
+  | H : _ |= _ |- _ => renames H to Hs
+  end.
+  rewrite Htrivial in Hs.
+  sep_cancel1 1 1.
+  instantiate (1 := Aemp).
+  eapply astar_emp_intro_r; eauto.
+
+  eapply sep_pure_l_intro; eauto.
+ 
+  eapply sep_pure_l_intro.
+  instantiate (1 := F).
+  instantiate (2 := id).
+  instantiate (1 := [[w7, w8, w9, w10, w11, w12, w13, $ 204]]).
+  split; eauto.
+  eapply match_end; eauto.
+ 
+  eapply sep_pure_l_intro.
+  instantiate (2 := [[id, w16, w17, w18, ct, ct +ᵢ ($ 84), w21, w22]]).
+  instantiate (1 := [[w23, w24, w25, w26, w27, w28, w29, w30]]).
+  eapply restore_end; eauto.
+
+  eapply sep_pure_l_intro.
+  simpl.
+  rewrite Int.sub_zero_l; eauto.
+  unfolds stack_frame_constraint.
+  simpls get_stk_addr.
+  simpls get_stk_cont.
+  eapply stk_fm_constraint_stable1 in Hst_fm_constraint; eauto.
+
+  eapply sep_pure_l_intro.
+  simpl.
+  repeat (split; eauto).
+  eapply rotate_end; eauto.
+
+  instantiate (1 := (cl, clfp)).
+  eapply astar_emp_elim_r.
+  eapply sep_pure_l_intro; eauto. 
+  destruct Hwin_save as [Hwin_save [Hcctx'_offset _] ].
+  split; eauto.
+  simpl. 
+  inversion Hst_fm_constraint; subst.
+  tryfalse.
+  match goal with
+  | H1 : get_frame_nth _ 6 = Some (get_stk_addr _), H2 : _ = get_stk_cont _  |- _ =>
+    renames H1 to Hpt, H2 to Hstk
+  end. 
+  clear - Hwin_save Hpt Hstk.
+  simpl in Hpt.
+  inversion Hpt; subst. 
+  unfold ctx_win_save in Hwin_save.
+  destruct cctx'.
+  unfold ctx_win_match in Hwin_save. 
+  destruct p.
+  destruct p.
+  destruct p.  
+  simpl in Hwin_save.
+  simpljoin1; subst.
+  unfold ctx_pt_stk.
+  simpl in Hstk.
+  subst.
+  simpls.
+  split; eauto.
+  split; eauto.
+  omega.
+
+  eexists.
+  instantiate (1 := nil).
+  simpl.
+  repeat (split; eauto).
+  
+  introv Hs.
+  unfold ta0_save_usedwindows_post in Hs.
+  sep_ex_elim_in Hs.
+  eapply sep_pure_l_elim in Hs.
+  destruct Hs as [Hlgvl1 Hs].
+  symmetry in Hlgvl1.
+  inversion Hlgvl1; subst.
+  sep_ex_intro.
+  eapply sep_pure_l_intro; eauto.
+  clear Hlgvl1.
+  do 12 sep_cancel1 1 1.
+  sep_cancel1 2 2.
+  sep_cancel1 2 2.
+
+  match goal with
+  | H : _ |= _ |- _ => renames H to Hs
+  end.
+  destruct Hwin_save as [Hwin_save [Hctx'_addr Hretl] ].
+  eapply sep_pure_l_elim in Hs.
+  destruct Hs as [Hstk_addr Hs].
+  eapply sep_pure_l_intro; eauto.
+  split.
+  rewrite Hct_ctx_offset.
+  rewrite Hctx'_addr.
+  eauto.
+  eauto.
+
+  eapply sep_pure_l_elim in Hs.
+  destruct Hs as [Hctsk Hs].
+  eapply sep_pure_l_intro; eauto.
+  introv Hct_neq.
+  eapply Hctsk in Hct_neq.
+  simpljoin1.
+  repeat (split; eauto).
+  eapply stk_fm_save_tail_stable1; eauto.
+Qed.
   
